bump to nightly-2023-02-03-15
mathlib commit https://github.com/leanprover-community/mathlib/commit/2705404e701abc6b3127da906f40bae062a169c9

Mathbin/Data/Finmap.lean
@@ -28,60 +28,78 @@ variable {α : Type u} {β : α → Type v}
 
 namespace Multiset
 
+#print Multiset.keys /-
 /-- Multiset of keys of an association multiset. -/
 def keys (s : Multiset (Sigma β)) : Multiset α :=
   s.map Sigma.fst
 #align multiset.keys Multiset.keys
+-/
 
+#print Multiset.coe_keys /-
 @[simp]
 theorem coe_keys {l : List (Sigma β)} : keys (l : Multiset (Sigma β)) = (l.keys : Multiset α) :=
   rfl
 #align multiset.coe_keys Multiset.coe_keys
+-/
 
+#print Multiset.NodupKeys /-
 /-- `nodupkeys s` means that `s` has no duplicate keys. -/
-def Nodupkeys (s : Multiset (Sigma β)) : Prop :=
+def NodupKeys (s : Multiset (Sigma β)) : Prop :=
   Quot.liftOn s List.NodupKeys fun s t p => propext <| perm_nodupKeys p
-#align multiset.nodupkeys Multiset.Nodupkeys
+#align multiset.nodupkeys Multiset.NodupKeys
+-/
 
+#print Multiset.coe_nodupKeys /-
 @[simp]
-theorem coe_nodupkeys {l : List (Sigma β)} : @Nodupkeys α β l ↔ l.NodupKeys :=
+theorem coe_nodupKeys {l : List (Sigma β)} : @NodupKeys α β l ↔ l.NodupKeys :=
   Iff.rfl
-#align multiset.coe_nodupkeys Multiset.coe_nodupkeys
+#align multiset.coe_nodupkeys Multiset.coe_nodupKeys
+-/
 
 end Multiset
 
 /-! ### finmap -/
 
 
+#print Finmap /-
 /-- `finmap β` is the type of finite maps over a multiset. It is effectively
   a quotient of `alist β` by permutation of the underlying list. -/
 structure Finmap (β : α → Type v) : Type max u v where
   entries : Multiset (Sigma β)
   NodupKeys : entries.NodupKeys
 #align finmap Finmap
+-/
 
+#print AList.toFinmap /-
 /-- The quotient map from `alist` to `finmap`. -/
 def AList.toFinmap (s : AList β) : Finmap β :=
   ⟨s.entries, s.NodupKeys⟩
 #align alist.to_finmap AList.toFinmap
+-/
 
 -- mathport name: to_finmap
 local notation:arg "⟦" a "⟧" => AList.toFinmap a
 
+#print AList.toFinmap_eq /-
 theorem AList.toFinmap_eq {s₁ s₂ : AList β} : ⟦s₁⟧ = ⟦s₂⟧ ↔ s₁.entries ~ s₂.entries := by
   cases s₁ <;> cases s₂ <;> simp [AList.toFinmap]
 #align alist.to_finmap_eq AList.toFinmap_eq
+-/
 
+#print AList.toFinmap_entries /-
 @[simp]
 theorem AList.toFinmap_entries (s : AList β) : ⟦s⟧.entries = s.entries :=
   rfl
 #align alist.to_finmap_entries AList.toFinmap_entries
+-/
 
+#print List.toFinmap /-
 /-- Given `l : list (sigma β)`, create a term of type `finmap β` by removing
 entries with duplicate keys. -/
 def List.toFinmap [DecidableEq α] (s : List (Sigma β)) : Finmap β :=
   s.toAList.toFinmap
 #align list.to_finmap List.toFinmap
+-/
 
 namespace Finmap
 
@@ -90,6 +108,7 @@ open AList
 /-! ### lifting from alist -/
 
 
+#print Finmap.liftOn /-
 /-- Lift a permutation-respecting function on `alist` to `finmap`. -/
 @[elab_as_elim]
 def liftOn {γ} (s : Finmap β) (f : AList β → γ)
@@ -105,12 +124,20 @@ def liftOn {γ} (s : Finmap β) (f : AList β → γ)
     rcases s.entries with ⟨l⟩
     exact id
 #align finmap.lift_on Finmap.liftOn
+-/
 
+/- warning: finmap.lift_on_to_finmap -> Finmap.liftOn_toFinmap is a dubious translation:
+lean 3 declaration is
+  forall {α : Type.{u1}} {β : α -> Type.{u2}} {γ : Type.{u3}} (s : AList.{u1, u2} α β) (f : (AList.{u1, u2} α β) -> γ) (H : forall (a : AList.{u1, u2} α β) (b : AList.{u1, u2} α β), (List.Perm.{max u1 u2} (Sigma.{u1, u2} α β) (AList.entries.{u1, u2} α β a) (AList.entries.{u1, u2} α β b)) -> (Eq.{succ u3} γ (f a) (f b))), Eq.{succ u3} γ (Finmap.liftOn.{u1, u2, u3} α β γ (AList.toFinmap.{u1, u2} α β s) f H) (f s)
+but is expected to have type
+  forall {α : Type.{u2}} {β : α -> Type.{u3}} {γ : Type.{u1}} (s : AList.{u2, u3} α β) (f : (AList.{u2, u3} α β) -> γ) (H : forall (a : AList.{u2, u3} α β) (b : AList.{u2, u3} α β), (List.Perm.{max u2 u3} (Sigma.{u2, u3} α β) (AList.entries.{u2, u3} α β a) (AList.entries.{u2, u3} α β b)) -> (Eq.{succ u1} γ (f a) (f b))), Eq.{succ u1} γ (Finmap.liftOn.{u2, u3, u1} α β γ (AList.toFinmap.{u2, u3} α β s) f H) (f s)
+Case conversion may be inaccurate. Consider using '#align finmap.lift_on_to_finmap Finmap.liftOn_toFinmapₓ'. -/
 @[simp]
 theorem liftOn_toFinmap {γ} (s : AList β) (f : AList β → γ) (H) : liftOn ⟦s⟧ f H = f s := by
   cases s <;> rfl
 #align finmap.lift_on_to_finmap Finmap.liftOn_toFinmap
 
+#print Finmap.liftOn₂ /-
 /-- Lift a permutation-respecting function on 2 `alist`s to 2 `finmap`s. -/
 @[elab_as_elim]
 def liftOn₂ {γ} (s₁ s₂ : Finmap β) (f : AList β → AList β → γ)
@@ -123,7 +150,14 @@ def liftOn₂ {γ} (s₁ s₂ : Finmap β) (f : AList β → AList β → γ)
     have H' : f a₁ = f a₂ := funext fun _ => H _ _ _ _ p (Perm.refl _)
     simp only [H']
 #align finmap.lift_on₂ Finmap.liftOn₂
+-/
 
+/- warning: finmap.lift_on₂_to_finmap -> Finmap.liftOn₂_toFinmap is a dubious translation:
+lean 3 declaration is
+  forall {α : Type.{u1}} {β : α -> Type.{u2}} {γ : Type.{u3}} (s₁ : AList.{u1, u2} α β) (s₂ : AList.{u1, u2} α β) (f : (AList.{u1, u2} α β) -> (AList.{u1, u2} α β) -> γ) (H : forall (a₁ : AList.{u1, u2} α β) (b₁ : AList.{u1, u2} α β) (a₂ : AList.{u1, u2} α β) (b₂ : AList.{u1, u2} α β), (List.Perm.{max u1 u2} (Sigma.{u1, u2} α β) (AList.entries.{u1, u2} α β a₁) (AList.entries.{u1, u2} α β a₂)) -> (List.Perm.{max u1 u2} (Sigma.{u1, u2} α β) (AList.entries.{u1, u2} α β b₁) (AList.entries.{u1, u2} α β b₂)) -> (Eq.{succ u3} γ (f a₁ b₁) (f a₂ b₂))), Eq.{succ u3} γ (Finmap.liftOn₂.{u1, u2, u3} α β γ (AList.toFinmap.{u1, u2} α β s₁) (AList.toFinmap.{u1, u2} α β s₂) f H) (f s₁ s₂)
+but is expected to have type
+  forall {α : Type.{u2}} {β : α -> Type.{u3}} {γ : Type.{u1}} (s₁ : AList.{u2, u3} α β) (s₂ : AList.{u2, u3} α β) (f : (AList.{u2, u3} α β) -> (AList.{u2, u3} α β) -> γ) (H : forall (a₁ : AList.{u2, u3} α β) (b₁ : AList.{u2, u3} α β) (a₂ : AList.{u2, u3} α β) (b₂ : AList.{u2, u3} α β), (List.Perm.{max u2 u3} (Sigma.{u2, u3} α β) (AList.entries.{u2, u3} α β a₁) (AList.entries.{u2, u3} α β a₂)) -> (List.Perm.{max u2 u3} (Sigma.{u2, u3} α β) (AList.entries.{u2, u3} α β b₁) (AList.entries.{u2, u3} α β b₂)) -> (Eq.{succ u1} γ (f a₁ b₁) (f a₂ b₂))), Eq.{succ u1} γ (Finmap.liftOn₂.{u2, u3, u1} α β γ (AList.toFinmap.{u2, u3} α β s₁) (AList.toFinmap.{u2, u3} α β s₂) f H) (f s₁ s₂)
+Case conversion may be inaccurate. Consider using '#align finmap.lift_on₂_to_finmap Finmap.liftOn₂_toFinmapₓ'. -/
 @[simp]
 theorem liftOn₂_toFinmap {γ} (s₁ s₂ : AList β) (f : AList β → AList β → γ) (H) :
     liftOn₂ ⟦s₁⟧ ⟦s₂⟧ f H = f s₁ s₂ := by cases s₁ <;> cases s₂ <;> rfl
@@ -132,35 +166,45 @@ theorem liftOn₂_toFinmap {γ} (s₁ s₂ : AList β) (f : AList β → AList �
 /-! ### induction -/
 
 
+#print Finmap.induction_on /-
 @[elab_as_elim]
 theorem induction_on {C : Finmap β → Prop} (s : Finmap β) (H : ∀ a : AList β, C ⟦a⟧) : C s := by
   rcases s with ⟨⟨a⟩, h⟩ <;> exact H ⟨a, h⟩
 #align finmap.induction_on Finmap.induction_on
+-/
 
+#print Finmap.induction_on₂ /-
 @[elab_as_elim]
 theorem induction_on₂ {C : Finmap β → Finmap β → Prop} (s₁ s₂ : Finmap β)
     (H : ∀ a₁ a₂ : AList β, C ⟦a₁⟧ ⟦a₂⟧) : C s₁ s₂ :=
   induction_on s₁ fun l₁ => induction_on s₂ fun l₂ => H l₁ l₂
 #align finmap.induction_on₂ Finmap.induction_on₂
+-/
 
+#print Finmap.induction_on₃ /-
 @[elab_as_elim]
 theorem induction_on₃ {C : Finmap β → Finmap β → Finmap β → Prop} (s₁ s₂ s₃ : Finmap β)
     (H : ∀ a₁ a₂ a₃ : AList β, C ⟦a₁⟧ ⟦a₂⟧ ⟦a₃⟧) : C s₁ s₂ s₃ :=
   induction_on₂ s₁ s₂ fun l₁ l₂ => induction_on s₃ fun l₃ => H l₁ l₂ l₃
 #align finmap.induction_on₃ Finmap.induction_on₃
+-/
 
 /-! ### extensionality -/
 
 
+#print Finmap.ext /-
 @[ext]
 theorem ext : ∀ {s t : Finmap β}, s.entries = t.entries → s = t
   | ⟨l₁, h₁⟩, ⟨l₂, h₂⟩, H => by congr
 #align finmap.ext Finmap.ext
+-/
 
+#print Finmap.ext_iff /-
 @[simp]
 theorem ext_iff {s t : Finmap β} : s.entries = t.entries ↔ s = t :=
   ⟨ext, congr_arg _⟩
 #align finmap.ext_iff Finmap.ext_iff
+-/
 
 /-! ### mem -/
 
@@ -169,36 +213,48 @@ theorem ext_iff {s t : Finmap β} : s.entries = t.entries ↔ s = t :=
 instance : Membership α (Finmap β) :=
   ⟨fun a s => a ∈ s.entries.keys⟩
 
+#print Finmap.mem_def /-
 theorem mem_def {a : α} {s : Finmap β} : a ∈ s ↔ a ∈ s.entries.keys :=
   Iff.rfl
 #align finmap.mem_def Finmap.mem_def
+-/
 
+#print Finmap.mem_toFinmap /-
 @[simp]
 theorem mem_toFinmap {a : α} {s : AList β} : a ∈ ⟦s⟧ ↔ a ∈ s :=
   Iff.rfl
 #align finmap.mem_to_finmap Finmap.mem_toFinmap
+-/
 
 /-! ### keys -/
 
 
+#print Finmap.keys /-
 /-- The set of keys of a finite map. -/
 def keys (s : Finmap β) : Finset α :=
   ⟨s.entries.keys, induction_on s keys_nodup⟩
 #align finmap.keys Finmap.keys
+-/
 
+#print Finmap.keys_val /-
 @[simp]
 theorem keys_val (s : AList β) : (keys ⟦s⟧).val = s.keys :=
   rfl
 #align finmap.keys_val Finmap.keys_val
+-/
 
+#print Finmap.keys_ext /-
 @[simp]
 theorem keys_ext {s₁ s₂ : AList β} : keys ⟦s₁⟧ = keys ⟦s₂⟧ ↔ s₁.keys ~ s₂.keys := by
   simp [keys, AList.keys]
 #align finmap.keys_ext Finmap.keys_ext
+-/
 
+#print Finmap.mem_keys /-
 theorem mem_keys {a : α} {s : Finmap β} : a ∈ s.keys ↔ a ∈ s :=
   induction_on s fun s => AList.mem_keys
 #align finmap.mem_keys Finmap.mem_keys
+-/
 
 /-! ### empty -/
 
@@ -210,99 +266,134 @@ instance : EmptyCollection (Finmap β) :=
 instance : Inhabited (Finmap β) :=
   ⟨∅⟩
 
+#print Finmap.empty_toFinmap /-
 @[simp]
 theorem empty_toFinmap : (⟦∅⟧ : Finmap β) = ∅ :=
   rfl
 #align finmap.empty_to_finmap Finmap.empty_toFinmap
+-/
 
+#print Finmap.toFinmap_nil /-
 @[simp]
 theorem toFinmap_nil [DecidableEq α] : ([].toFinmap : Finmap β) = ∅ :=
   rfl
 #align finmap.to_finmap_nil Finmap.toFinmap_nil
+-/
 
+#print Finmap.not_mem_empty /-
 theorem not_mem_empty {a : α} : a ∉ (∅ : Finmap β) :=
   Multiset.not_mem_zero a
 #align finmap.not_mem_empty Finmap.not_mem_empty
+-/
 
+#print Finmap.keys_empty /-
 @[simp]
 theorem keys_empty : (∅ : Finmap β).keys = ∅ :=
   rfl
 #align finmap.keys_empty Finmap.keys_empty
+-/
 
 /-! ### singleton -/
 
 
+#print Finmap.singleton /-
 /-- The singleton map. -/
 def singleton (a : α) (b : β a) : Finmap β :=
   ⟦AList.singleton a b⟧
 #align finmap.singleton Finmap.singleton
+-/
 
+#print Finmap.keys_singleton /-
 @[simp]
 theorem keys_singleton (a : α) (b : β a) : (singleton a b).keys = {a} :=
   rfl
 #align finmap.keys_singleton Finmap.keys_singleton
+-/
 
+#print Finmap.mem_singleton /-
 @[simp]
 theorem mem_singleton (x y : α) (b : β y) : x ∈ singleton y b ↔ x = y := by
   simp only [singleton] <;> erw [mem_cons_eq, mem_nil_iff, or_false_iff]
 #align finmap.mem_singleton Finmap.mem_singleton
+-/
 
 section
 
 variable [DecidableEq α]
 
+#print Finmap.hasDecidableEq /-
 instance hasDecidableEq [∀ a, DecidableEq (β a)] : DecidableEq (Finmap β)
   | s₁, s₂ => decidable_of_iff _ ext_iff
 #align finmap.has_decidable_eq Finmap.hasDecidableEq
+-/
 
 /-! ### lookup -/
 
 
+#print Finmap.lookup /-
 /-- Look up the value associated to a key in a map. -/
 def lookup (a : α) (s : Finmap β) : Option (β a) :=
   liftOn s (lookup a) fun s t => perm_lookup
 #align finmap.lookup Finmap.lookup
+-/
 
+#print Finmap.lookup_toFinmap /-
 @[simp]
 theorem lookup_toFinmap (a : α) (s : AList β) : lookup a ⟦s⟧ = s.dlookup a :=
   rfl
 #align finmap.lookup_to_finmap Finmap.lookup_toFinmap
+-/
 
+#print Finmap.dlookup_list_toFinmap /-
 @[simp]
-theorem lookup_list_toFinmap (a : α) (s : List (Sigma β)) : lookup a s.toFinmap = s.dlookup a := by
+theorem dlookup_list_toFinmap (a : α) (s : List (Sigma β)) : lookup a s.toFinmap = s.dlookup a := by
   rw [List.toFinmap, lookup_to_finmap, lookup_to_alist]
-#align finmap.lookup_list_to_finmap Finmap.lookup_list_toFinmap
+#align finmap.lookup_list_to_finmap Finmap.dlookup_list_toFinmap
+-/
 
+#print Finmap.lookup_empty /-
 @[simp]
 theorem lookup_empty (a) : lookup a (∅ : Finmap β) = none :=
   rfl
 #align finmap.lookup_empty Finmap.lookup_empty
+-/
 
+#print Finmap.lookup_isSome /-
 theorem lookup_isSome {a : α} {s : Finmap β} : (s.dlookup a).isSome ↔ a ∈ s :=
   induction_on s fun s => AList.lookup_isSome
 #align finmap.lookup_is_some Finmap.lookup_isSome
+-/
 
+#print Finmap.lookup_eq_none /-
 theorem lookup_eq_none {a} {s : Finmap β} : lookup a s = none ↔ a ∉ s :=
   induction_on s fun s => AList.lookup_eq_none
 #align finmap.lookup_eq_none Finmap.lookup_eq_none
+-/
 
+#print Finmap.lookup_singleton_eq /-
 @[simp]
 theorem lookup_singleton_eq {a : α} {b : β a} : (singleton a b).dlookup a = some b := by
   rw [singleton, lookup_to_finmap, AList.singleton, AList.lookup, lookup_cons_eq]
 #align finmap.lookup_singleton_eq Finmap.lookup_singleton_eq
+-/
 
 instance (a : α) (s : Finmap β) : Decidable (a ∈ s) :=
   decidable_of_iff _ lookup_isSome
 
+#print Finmap.mem_iff /-
 theorem mem_iff {a : α} {s : Finmap β} : a ∈ s ↔ ∃ b, s.dlookup a = some b :=
   induction_on s fun s =>
     Iff.trans List.mem_keys <| exists_congr fun b => (mem_lookup_iff s.NodupKeys).symm
 #align finmap.mem_iff Finmap.mem_iff
+-/
 
+#print Finmap.mem_of_lookup_eq_some /-
 theorem mem_of_lookup_eq_some {a : α} {b : β a} {s : Finmap β} (h : s.dlookup a = some b) : a ∈ s :=
   mem_iff.mpr ⟨_, h⟩
 #align finmap.mem_of_lookup_eq_some Finmap.mem_of_lookup_eq_some
+-/
 
+#print Finmap.ext_lookup /-
 theorem ext_lookup {s₁ s₂ : Finmap β} : (∀ x, s₁.dlookup x = s₂.dlookup x) → s₁ = s₂ :=
   induction_on₂ s₁ s₂ fun s₁ s₂ h =>
     by
@@ -312,42 +403,54 @@ theorem ext_lookup {s₁ s₂ : Finmap β} : (∀ x, s₁.dlookup x = s₂.dlook
     intro x y
     rw [h]
 #align finmap.ext_lookup Finmap.ext_lookup
+-/
 
 /-! ### replace -/
 
 
+#print Finmap.replace /-
 /-- Replace a key with a given value in a finite map.
   If the key is not present it does nothing. -/
 def replace (a : α) (b : β a) (s : Finmap β) : Finmap β :=
   liftOn s (fun t => ⟦replace a b t⟧) fun s₁ s₂ p => toFinmap_eq.2 <| perm_replace p
 #align finmap.replace Finmap.replace
+-/
 
+#print Finmap.replace_toFinmap /-
 @[simp]
 theorem replace_toFinmap (a : α) (b : β a) (s : AList β) : replace a b ⟦s⟧ = ⟦s.replace a b⟧ := by
   simp [replace]
 #align finmap.replace_to_finmap Finmap.replace_toFinmap
+-/
 
+#print Finmap.keys_replace /-
 @[simp]
 theorem keys_replace (a : α) (b : β a) (s : Finmap β) : (replace a b s).keys = s.keys :=
   induction_on s fun s => by simp
 #align finmap.keys_replace Finmap.keys_replace
+-/
 
+#print Finmap.mem_replace /-
 @[simp]
 theorem mem_replace {a a' : α} {b : β a} {s : Finmap β} : a' ∈ replace a b s ↔ a' ∈ s :=
   induction_on s fun s => by simp
 #align finmap.mem_replace Finmap.mem_replace
+-/
 
 end
 
 /-! ### foldl -/
 
 
+#print Finmap.foldl /-
 /-- Fold a commutative function over the key-value pairs in the map -/
 def foldl {δ : Type w} (f : δ → ∀ a, β a → δ)
     (H : ∀ d a₁ b₁ a₂ b₂, f (f d a₁ b₁) a₂ b₂ = f (f d a₂ b₂) a₁ b₁) (d : δ) (m : Finmap β) : δ :=
   m.entries.foldl (fun d s => f d s.1 s.2) (fun d s t => H _ _ _ _ _) d
 #align finmap.foldl Finmap.foldl
+-/
 
+#print Finmap.any /-
 /-- `any f s` returns `tt` iff there exists a value `v` in `s` such that `f v = tt`. -/
 def any (f : ∀ x, β x → Bool) (s : Finmap β) : Bool :=
   s.foldl (fun x y z => x ∨ f y z)
@@ -356,7 +459,9 @@ def any (f : ∀ x, β x → Bool) (s : Finmap β) : Bool :=
       simp [or_right_comm])
     false
 #align finmap.any Finmap.any
+-/
 
+#print Finmap.all /-
 /-- `all f s` returns `tt` iff `f v = tt` for all values `v` in `s`. -/
 def all (f : ∀ x, β x → Bool) (s : Finmap β) : Bool :=
   s.foldl (fun x y z => x ∧ f y z)
@@ -365,6 +470,7 @@ def all (f : ∀ x, β x → Bool) (s : Finmap β) : Bool :=
       simp [and_right_comm])
     false
 #align finmap.all Finmap.all
+-/
 
 /-! ### erase -/
 
@@ -373,56 +479,76 @@ section
 
 variable [DecidableEq α]
 
+#print Finmap.erase /-
 /-- Erase a key from the map. If the key is not present it does nothing. -/
 def erase (a : α) (s : Finmap β) : Finmap β :=
   liftOn s (fun t => ⟦erase a t⟧) fun s₁ s₂ p => toFinmap_eq.2 <| perm_erase p
 #align finmap.erase Finmap.erase
+-/
 
+#print Finmap.erase_toFinmap /-
 @[simp]
 theorem erase_toFinmap (a : α) (s : AList β) : erase a ⟦s⟧ = ⟦s.eraseₓ a⟧ := by simp [erase]
 #align finmap.erase_to_finmap Finmap.erase_toFinmap
+-/
 
+#print Finmap.keys_erase_toFinset /-
 @[simp]
-theorem keys_erase_to_finset (a : α) (s : AList β) : keys ⟦s.eraseₓ a⟧ = (keys ⟦s⟧).eraseₓ a := by
+theorem keys_erase_toFinset (a : α) (s : AList β) : keys ⟦s.eraseₓ a⟧ = (keys ⟦s⟧).eraseₓ a := by
   simp [Finset.erase, keys, AList.erase, keys_kerase]
-#align finmap.keys_erase_to_finset Finmap.keys_erase_to_finset
+#align finmap.keys_erase_to_finset Finmap.keys_erase_toFinset
+-/
 
+#print Finmap.keys_erase /-
 @[simp]
 theorem keys_erase (a : α) (s : Finmap β) : (erase a s).keys = s.keys.eraseₓ a :=
   induction_on s fun s => by simp
 #align finmap.keys_erase Finmap.keys_erase
+-/
 
+#print Finmap.mem_erase /-
 @[simp]
 theorem mem_erase {a a' : α} {s : Finmap β} : a' ∈ erase a s ↔ a' ≠ a ∧ a' ∈ s :=
   induction_on s fun s => by simp
 #align finmap.mem_erase Finmap.mem_erase
+-/
 
+#print Finmap.not_mem_erase_self /-
 theorem not_mem_erase_self {a : α} {s : Finmap β} : ¬a ∈ erase a s := by
   rw [mem_erase, not_and_or, Classical.not_not] <;> left <;> rfl
 #align finmap.not_mem_erase_self Finmap.not_mem_erase_self
+-/
 
+#print Finmap.lookup_erase /-
 @[simp]
 theorem lookup_erase (a) (s : Finmap β) : lookup a (erase a s) = none :=
   induction_on s <| lookup_erase a
 #align finmap.lookup_erase Finmap.lookup_erase
+-/
 
+#print Finmap.lookup_erase_ne /-
 @[simp]
 theorem lookup_erase_ne {a a'} {s : Finmap β} (h : a ≠ a') : lookup a (erase a' s) = lookup a s :=
   induction_on s fun s => lookup_erase_ne h
 #align finmap.lookup_erase_ne Finmap.lookup_erase_ne
+-/
 
+#print Finmap.erase_erase /-
 theorem erase_erase {a a' : α} {s : Finmap β} : erase a (erase a' s) = erase a' (erase a s) :=
   induction_on s fun s => ext (by simp only [erase_erase, erase_to_finmap])
 #align finmap.erase_erase Finmap.erase_erase
+-/
 
 /-! ### sdiff -/
 
 
+#print Finmap.sdiff /-
 /-- `sdiff s s'` consists of all key-value pairs from `s` and `s'` where the keys are in `s` or
 `s'` but not both. -/
 def sdiff (s s' : Finmap β) : Finmap β :=
   s'.foldl (fun s x _ => s.eraseₓ x) (fun a₀ a₁ _ a₂ _ => erase_erase) s
 #align finmap.sdiff Finmap.sdiff
+-/
 
 instance : SDiff (Finmap β) :=
   ⟨sdiff⟩
@@ -430,55 +556,74 @@ instance : SDiff (Finmap β) :=
 /-! ### insert -/
 
 
+#print Finmap.insert /-
 /-- Insert a key-value pair into a finite map, replacing any existing pair with
   the same key. -/
 def insert (a : α) (b : β a) (s : Finmap β) : Finmap β :=
   liftOn s (fun t => ⟦insert a b t⟧) fun s₁ s₂ p => toFinmap_eq.2 <| perm_insert p
 #align finmap.insert Finmap.insert
+-/
 
+#print Finmap.insert_toFinmap /-
 @[simp]
 theorem insert_toFinmap (a : α) (b : β a) (s : AList β) : insert a b ⟦s⟧ = ⟦s.insert a b⟧ := by
   simp [insert]
 #align finmap.insert_to_finmap Finmap.insert_toFinmap
+-/
 
+#print Finmap.insert_entries_of_neg /-
 theorem insert_entries_of_neg {a : α} {b : β a} {s : Finmap β} :
     a ∉ s → (insert a b s).entries = ⟨a, b⟩ ::ₘ s.entries :=
   induction_on s fun s h => by simp [insert_entries_of_neg (mt mem_to_finmap.1 h)]
 #align finmap.insert_entries_of_neg Finmap.insert_entries_of_neg
+-/
 
+#print Finmap.mem_insert /-
 @[simp]
 theorem mem_insert {a a' : α} {b' : β a'} {s : Finmap β} : a ∈ insert a' b' s ↔ a = a' ∨ a ∈ s :=
   induction_on s mem_insert
 #align finmap.mem_insert Finmap.mem_insert
+-/
 
+#print Finmap.lookup_insert /-
 @[simp]
 theorem lookup_insert {a} {b : β a} (s : Finmap β) : lookup a (insert a b s) = some b :=
   induction_on s fun s => by simp only [insert_to_finmap, lookup_to_finmap, lookup_insert]
 #align finmap.lookup_insert Finmap.lookup_insert
+-/
 
+#print Finmap.lookup_insert_of_ne /-
 @[simp]
 theorem lookup_insert_of_ne {a a'} {b : β a} (s : Finmap β) (h : a' ≠ a) :
     lookup a' (insert a b s) = lookup a' s :=
   induction_on s fun s => by simp only [insert_to_finmap, lookup_to_finmap, lookup_insert_ne h]
 #align finmap.lookup_insert_of_ne Finmap.lookup_insert_of_ne
+-/
 
+#print Finmap.insert_insert /-
 @[simp]
 theorem insert_insert {a} {b b' : β a} (s : Finmap β) :
     (s.insert a b).insert a b' = s.insert a b' :=
   induction_on s fun s => by simp only [insert_to_finmap, insert_insert]
 #align finmap.insert_insert Finmap.insert_insert
+-/
 
+#print Finmap.insert_insert_of_ne /-
 theorem insert_insert_of_ne {a a'} {b : β a} {b' : β a'} (s : Finmap β) (h : a ≠ a') :
     (s.insert a b).insert a' b' = (s.insert a' b').insert a b :=
   induction_on s fun s => by
     simp only [insert_to_finmap, AList.toFinmap_eq, insert_insert_of_ne _ h]
 #align finmap.insert_insert_of_ne Finmap.insert_insert_of_ne
+-/
 
+#print Finmap.toFinmap_cons /-
 theorem toFinmap_cons (a : α) (b : β a) (xs : List (Sigma β)) :
     List.toFinmap (⟨a, b⟩ :: xs) = insert a b xs.toFinmap :=
   rfl
 #align finmap.to_finmap_cons Finmap.toFinmap_cons
+-/
 
+#print Finmap.mem_list_toFinmap /-
 theorem mem_list_toFinmap (a : α) (xs : List (Sigma β)) :
     a ∈ xs.toFinmap ↔ ∃ b : β a, Sigma.mk a b ∈ xs :=
   by
@@ -493,62 +638,82 @@ theorem mem_list_toFinmap (a : α) (xs : List (Sigma β)) :
   rintro ⟨⟩
   simp only [exists_eq, heq_iff_eq]
 #align finmap.mem_list_to_finmap Finmap.mem_list_toFinmap
+-/
 
+#print Finmap.insert_singleton_eq /-
 @[simp]
 theorem insert_singleton_eq {a : α} {b b' : β a} : insert a b (singleton a b') = singleton a b := by
   simp only [singleton, Finmap.insert_toFinmap, AList.insert_singleton_eq]
 #align finmap.insert_singleton_eq Finmap.insert_singleton_eq
+-/
 
 /-! ### extract -/
 
 
+#print Finmap.extract /-
 /-- Erase a key from the map, and return the corresponding value, if found. -/
 def extract (a : α) (s : Finmap β) : Option (β a) × Finmap β :=
   liftOn s (fun t => Prod.map id toFinmap (extract a t)) fun s₁ s₂ p => by
     simp [perm_lookup p, to_finmap_eq, perm_erase p]
 #align finmap.extract Finmap.extract
+-/
 
+#print Finmap.extract_eq_lookup_erase /-
 @[simp]
 theorem extract_eq_lookup_erase (a : α) (s : Finmap β) : extract a s = (lookup a s, erase a s) :=
   induction_on s fun s => by simp [extract]
 #align finmap.extract_eq_lookup_erase Finmap.extract_eq_lookup_erase
+-/
 
 /-! ### union -/
 
 
+#print Finmap.union /-
 /-- `s₁ ∪ s₂` is the key-based union of two finite maps. It is left-biased: if
 there exists an `a ∈ s₁`, `lookup a (s₁ ∪ s₂) = lookup a s₁`. -/
 def union (s₁ s₂ : Finmap β) : Finmap β :=
   liftOn₂ s₁ s₂ (fun s₁ s₂ => ⟦s₁ ∪ s₂⟧) fun s₁ s₂ s₃ s₄ p₁₃ p₂₄ =>
     toFinmap_eq.mpr <| perm_union p₁₃ p₂₄
 #align finmap.union Finmap.union
+-/
 
 instance : Union (Finmap β) :=
   ⟨union⟩
 
+#print Finmap.mem_union /-
 @[simp]
 theorem mem_union {a} {s₁ s₂ : Finmap β} : a ∈ s₁ ∪ s₂ ↔ a ∈ s₁ ∨ a ∈ s₂ :=
   induction_on₂ s₁ s₂ fun _ _ => mem_union
 #align finmap.mem_union Finmap.mem_union
+-/
 
+#print Finmap.union_toFinmap /-
 @[simp]
 theorem union_toFinmap (s₁ s₂ : AList β) : ⟦s₁⟧ ∪ ⟦s₂⟧ = ⟦s₁ ∪ s₂⟧ := by simp [(· ∪ ·), union]
 #align finmap.union_to_finmap Finmap.union_toFinmap
+-/
 
+#print Finmap.keys_union /-
 theorem keys_union {s₁ s₂ : Finmap β} : (s₁ ∪ s₂).keys = s₁.keys ∪ s₂.keys :=
   induction_on₂ s₁ s₂ fun s₁ s₂ => Finset.ext <| by simp [keys]
 #align finmap.keys_union Finmap.keys_union
+-/
 
+#print Finmap.lookup_union_left /-
 @[simp]
 theorem lookup_union_left {a} {s₁ s₂ : Finmap β} : a ∈ s₁ → lookup a (s₁ ∪ s₂) = lookup a s₁ :=
   induction_on₂ s₁ s₂ fun s₁ s₂ => lookup_union_left
 #align finmap.lookup_union_left Finmap.lookup_union_left
+-/
 
+#print Finmap.lookup_union_right /-
 @[simp]
 theorem lookup_union_right {a} {s₁ s₂ : Finmap β} : a ∉ s₁ → lookup a (s₁ ∪ s₂) = lookup a s₂ :=
   induction_on₂ s₁ s₂ fun s₁ s₂ => lookup_union_right
 #align finmap.lookup_union_right Finmap.lookup_union_right
+-/
 
+#print Finmap.lookup_union_left_of_not_in /-
 theorem lookup_union_left_of_not_in {a} {s₁ s₂ : Finmap β} (h : a ∉ s₂) :
     lookup a (s₁ ∪ s₂) = lookup a s₁ :=
   by
@@ -556,41 +721,55 @@ theorem lookup_union_left_of_not_in {a} {s₁ s₂ : Finmap β} (h : a ∉ s₂)
   · rw [lookup_union_left h']
   · rw [lookup_union_right h', lookup_eq_none.mpr h, lookup_eq_none.mpr h']
 #align finmap.lookup_union_left_of_not_in Finmap.lookup_union_left_of_not_in
+-/
 
+#print Finmap.mem_lookup_union /-
 @[simp]
 theorem mem_lookup_union {a} {b : β a} {s₁ s₂ : Finmap β} :
     b ∈ lookup a (s₁ ∪ s₂) ↔ b ∈ lookup a s₁ ∨ a ∉ s₁ ∧ b ∈ lookup a s₂ :=
   induction_on₂ s₁ s₂ fun s₁ s₂ => mem_lookup_union
 #align finmap.mem_lookup_union Finmap.mem_lookup_union
+-/
 
+#print Finmap.mem_lookup_union_middle /-
 theorem mem_lookup_union_middle {a} {b : β a} {s₁ s₂ s₃ : Finmap β} :
     b ∈ lookup a (s₁ ∪ s₃) → a ∉ s₂ → b ∈ lookup a (s₁ ∪ s₂ ∪ s₃) :=
   induction_on₃ s₁ s₂ s₃ fun s₁ s₂ s₃ => mem_lookup_union_middle
 #align finmap.mem_lookup_union_middle Finmap.mem_lookup_union_middle
+-/
 
+#print Finmap.insert_union /-
 theorem insert_union {a} {b : β a} {s₁ s₂ : Finmap β} : insert a b (s₁ ∪ s₂) = insert a b s₁ ∪ s₂ :=
   induction_on₂ s₁ s₂ fun a₁ a₂ => by simp [insert_union]
 #align finmap.insert_union Finmap.insert_union
+-/
 
+#print Finmap.union_assoc /-
 theorem union_assoc {s₁ s₂ s₃ : Finmap β} : s₁ ∪ s₂ ∪ s₃ = s₁ ∪ (s₂ ∪ s₃) :=
   induction_on₃ s₁ s₂ s₃ fun s₁ s₂ s₃ => by
     simp only [AList.toFinmap_eq, union_to_finmap, AList.union_assoc]
 #align finmap.union_assoc Finmap.union_assoc
+-/
 
+#print Finmap.empty_union /-
 @[simp]
 theorem empty_union {s₁ : Finmap β} : ∅ ∪ s₁ = s₁ :=
   induction_on s₁ fun s₁ => by
     rw [← empty_to_finmap] <;>
       simp [-empty_to_finmap, AList.toFinmap_eq, union_to_finmap, AList.union_assoc]
 #align finmap.empty_union Finmap.empty_union
+-/
 
+#print Finmap.union_empty /-
 @[simp]
 theorem union_empty {s₁ : Finmap β} : s₁ ∪ ∅ = s₁ :=
   induction_on s₁ fun s₁ => by
     rw [← empty_to_finmap] <;>
       simp [-empty_to_finmap, AList.toFinmap_eq, union_to_finmap, AList.union_assoc]
 #align finmap.union_empty Finmap.union_empty
+-/
 
+#print Finmap.erase_union_singleton /-
 theorem erase_union_singleton (a : α) (b : β a) (s : Finmap β) (h : s.dlookup a = some b) :
     s.eraseₓ a ∪ singleton a b = s :=
   ext_lookup fun x => by
@@ -600,28 +779,37 @@ theorem erase_union_singleton (a : α) (b : β a) (s : Finmap β) (h : s.dlookup
     · have : x ∉ singleton a b := by rwa [mem_singleton]
       rw [lookup_union_left_of_not_in this, lookup_erase_ne h']
 #align finmap.erase_union_singleton Finmap.erase_union_singleton
+-/
 
 end
 
 /-! ### disjoint -/
 
 
+#print Finmap.Disjoint /-
 /-- `disjoint s₁ s₂` holds if `s₁` and `s₂` have no keys in common. -/
 def Disjoint (s₁ s₂ : Finmap β) : Prop :=
   ∀ x ∈ s₁, ¬x ∈ s₂
 #align finmap.disjoint Finmap.Disjoint
+-/
 
+#print Finmap.disjoint_empty /-
 theorem disjoint_empty (x : Finmap β) : Disjoint ∅ x :=
   fun.
 #align finmap.disjoint_empty Finmap.disjoint_empty
+-/
 
+#print Finmap.Disjoint.symm /-
 @[symm]
 theorem Disjoint.symm (x y : Finmap β) (h : Disjoint x y) : Disjoint y x := fun p hy hx => h p hx hy
 #align finmap.disjoint.symm Finmap.Disjoint.symm
+-/
 
+#print Finmap.Disjoint.symm_iff /-
 theorem Disjoint.symm_iff (x y : Finmap β) : Disjoint x y ↔ Disjoint y x :=
   ⟨Disjoint.symm x y, Disjoint.symm y x⟩
 #align finmap.disjoint.symm_iff Finmap.Disjoint.symm_iff
+-/
 
 section
 
@@ -629,21 +817,28 @@ variable [DecidableEq α]
 
 instance : DecidableRel (@Disjoint α β) := fun x y => by dsimp only [Disjoint] <;> infer_instance
 
+#print Finmap.disjoint_union_left /-
 theorem disjoint_union_left (x y z : Finmap β) : Disjoint (x ∪ y) z ↔ Disjoint x z ∧ Disjoint y z :=
   by simp [Disjoint, Finmap.mem_union, or_imp, forall_and]
 #align finmap.disjoint_union_left Finmap.disjoint_union_left
+-/
 
+#print Finmap.disjoint_union_right /-
 theorem disjoint_union_right (x y z : Finmap β) :
     Disjoint x (y ∪ z) ↔ Disjoint x y ∧ Disjoint x z := by
   rw [disjoint.symm_iff, disjoint_union_left, disjoint.symm_iff _ x, disjoint.symm_iff _ x]
 #align finmap.disjoint_union_right Finmap.disjoint_union_right
+-/
 
+#print Finmap.union_comm_of_disjoint /-
 theorem union_comm_of_disjoint {s₁ s₂ : Finmap β} : Disjoint s₁ s₂ → s₁ ∪ s₂ = s₂ ∪ s₁ :=
   induction_on₂ s₁ s₂ fun s₁ s₂ => by
     intro h
     simp only [AList.toFinmap_eq, union_to_finmap, AList.union_comm_of_disjoint h]
 #align finmap.union_comm_of_disjoint Finmap.union_comm_of_disjoint
+-/
 
+#print Finmap.union_cancel /-
 theorem union_cancel {s₁ s₂ s₃ : Finmap β} (h : Disjoint s₁ s₃) (h' : Disjoint s₂ s₃) :
     s₁ ∪ s₃ = s₂ ∪ s₃ ↔ s₁ = s₂ :=
   ⟨fun h'' => by
@@ -656,6 +851,7 @@ theorem union_cancel {s₁ s₂ s₃ : Finmap β} (h : Disjoint s₁ s₃) (h' :
       · rwa [lookup_union_left_of_not_in (h' _ hs₂), lookup_union_left hs₂] at this
       · rw [lookup_eq_none.mpr hs₁, lookup_eq_none.mpr hs₂], fun h => h ▸ rfl⟩
 #align finmap.union_cancel Finmap.union_cancel
+-/
 
 end
 
